slight simplifications to client

theories/iris/examples/effects/generator_client.v
@@ -45,8 +45,8 @@ Section GeneratorClient.
   Context `{!wasmG Σ, !hvisG Σ, !hmsG Σ, !hasG Σ}.
   Context `{!inG Σ (excl_authR (listO (leibnizO i32)))}.
 
-  Definition sum_until_client generator_exp_addr sum_until_exp_addr mod_addr n :=
-    [ ID_instantiate [ generator_exp_addr; sum_until_exp_addr ] mod_addr [];
+  Definition sum_until_client sum_until_exp_addr mod_addr n :=
+    [ ID_instantiate [ sum_until_exp_addr ] mod_addr [];
 H_invoke sum_until_exp_addr [VAL_int32 n]
     ].
 
@@ -54,13 +54,12 @@ H_invoke sum_until_exp_addr [VAL_int32 n]
     (□ ∀ Φ, P -∗ (∀ v, Q -∗ Φ v) -∗ WP (es : host_expr) @ NotStuck ; ⊤ {{ v, Φ v }})%I (at level 50).
 
 
-  Lemma instantiate_client naturals_exp_addr sum_until_exp_addr mod_addr n :
+  Lemma instantiate_client sum_until_exp_addr mod_addr n :
     ⊢ {{{{
         mod_addr ↪[mods] generator_module ∗
-        (∃ exp1, naturals_exp_addr ↪[vis] exp1) ∗
-        (∃ exp2, sum_until_exp_addr ↪[vis] exp2)
+        (∃ exp, sum_until_exp_addr ↪[vis] exp)
       }}}}
-        ((sum_until_client naturals_exp_addr sum_until_exp_addr mod_addr n, [], empty_frame) : host_expr)
+        ((sum_until_client sum_until_exp_addr mod_addr n, [], empty_frame) : host_expr)
       {{{{ w, ⌜w = (immHV [VAL_num (VAL_int32 $ Sum_until_i32 n)], empty_frame)⌝ }}}}.
   Proof.
     iIntros "!>" (Φ) "(Hmod & Hexp1 & Hexp2 ) HΦ".
